\documentclass{article}
\usepackage{epsfig}
\pagestyle{empty}
\begin{document}
$ a < x < b $
\pagebreak

$ f(a) > f(x) < f(b) $
\pagebreak

$b$
\pagebreak

\[ g(a) = \Vec{s} + a \Vec{d} \]
\pagebreak

$f(x),\ x>0$
\pagebreak

$x$
\pagebreak

$f(x)$
\pagebreak

$\Vec{s}$
\pagebreak

$\Vec{d}$
\pagebreak

$f(\cdotp)$
\pagebreak

$f(\vec{s} + x\vec{d})$
\pagebreak

$x_\mathrm{optimal} = 0$
\pagebreak

$*100$
\pagebreak

$\nabla f(x)$
\pagebreak

$h$
\pagebreak

$h_i$
\pagebreak

$ y_i = f(h_i)$
\pagebreak

\[ \begin{array}{ccccccc} h_0 & y_0 & P_0 & & & \\ & & & P_{01} & & \\ h_1 & y_1 & P_1 & & P_{012} & \\ & & & P_{12} & & P_{0123} \\ h_2 & y_2 & P_2 & & P_{123} & \\ & & & P_{23} & & \\ h_3 & y_3 & P_3 & & & \\ \end{array} \]
\pagebreak

$P_{123}$
\pagebreak

$ h$
\pagebreak

$P_i = y_i = f(h_i)$
\pagebreak

\begin{equation} P_{k\cdots n} = \frac{(h - h_n)P_{k \cdots n-1} + (h_k - h)P_{k+1 \cdots n}}{h_k - h_n} \end{equation}
\pagebreak

$ h=0 $
\pagebreak

$ h_i = c^{-i} $
\pagebreak

$ c $
\pagebreak

\[ P_{k \cdots n} = \frac{c^{-k} P_{k+1 \cdots n} - P_{k \cdots n-1}}{c^{n - k} - 1} \]
\pagebreak

$P_{234}$
\pagebreak

$P_{34}$
\pagebreak

$P_{23}$
\pagebreak

$ t $
\pagebreak

$ c = 1.1 $
\pagebreak

$ t = 2 $
\pagebreak

\[ \frac{\partial^2 f}{\partial x^2} \approx \frac{f(x-h) - 2f(x) + f(x+h)}{h^2} \]
\pagebreak

\[ \frac{\partial^2 f}{\partial x\partial y} \approx \frac{f(x+h, y+h) - f(x-h,y+h) - f(x+h, y-h) + f(x-h, y-h)}{4h^2} \]
\pagebreak

$N+1$
\pagebreak

$f$
\pagebreak

$x_w$
\pagebreak

$x_0$
\pagebreak

$v = x_0 - x_w$
\pagebreak

$ x_r = x_0 + \alpha v$
\pagebreak

$f(x_r)$
\pagebreak

$x_e = x_0 + \rho \alpha v $
\pagebreak

$x_e$
\pagebreak

$x_r$
\pagebreak

$x_c = x_0 + \gamma v$
\pagebreak

$f(x_c) < f(x_r)$
\pagebreak

$x_c$
\pagebreak

$\sigma$
\pagebreak

$\alpha = 1$
\pagebreak

$\rho = 2$
\pagebreak

$\gamma = 1/2$
\pagebreak

$\sigma = 1/2$
\pagebreak

$[A | I ]$
\pagebreak

$[ I | A^{-1}]$
\pagebreak

$Ax = b$
\pagebreak

$A$
\pagebreak

$ a < b < c $
\pagebreak

$ f(a) > f(b) < f(c) $
\pagebreak

$M^{\dagger}A$
\pagebreak

$M^{\dagger}b$
\pagebreak

$M^{\dagger}$
\pagebreak

$L_2$
\pagebreak

$L_2^2$
\pagebreak

$L_1$
\pagebreak

$L_\infty$
\pagebreak

$\hat{v}$
\pagebreak

$[v_1, v_2, \cdots, v_{i-1}] / v_i $
\pagebreak

$[v_1, v_2, \cdots, v_{i}, 1]$
\pagebreak

$ \frac{m + m^{\mathsf T}}{2} $
\pagebreak

$p = (x,y)$
\pagebreak

$q = ( \operatorname{round}\ x, \operatorname{round}\ y)$
\pagebreak

$v$
\pagebreak

$v = I(q)$
\pagebreak

$p' = ( \operatorname{floor}\ x, \operatorname{floor}\ y)$
\pagebreak

$\delta = p - p'$
\pagebreak

$p'$
\pagebreak

\[\begin{array}{rl} a =& I(p')\\ b =& I(p' + (1,0))\\ c =& I(p' + (0,1))\\ d =& I(p' + (1,1)) \end{array} \]
\pagebreak

\[v = (1-\delta_y)((1-\delta_x)a + \delta_xb) + \delta_y((1-\delta_x)c + \delta_xd)\]
\pagebreak

\[ v = \sum_{m=-1}^2\sum_{n=-1}^2 I(x' + m, y' + n)r(m - \delta_x)r(\delta_y-n) \]
\pagebreak

\[\begin{array}{rl} r(x) =& \frac{1}{6}\left[ p(x+2)^3 - 4p(x+1)^3 + 6p(x)^3 - 4p(x-1)^3 \right]\\ p(x) =& \begin{cases}x&x>0\\0&x \le 0\end{cases} \end{array}\]
\pagebreak

$w(x)=\frac{1}{\sigma + |x|}$
\pagebreak

$w(x)=\frac{1}{\sigma + x^2}$
\pagebreak

$w(x)=1$
\pagebreak

$w(x)$
\pagebreak

$w(x) + xw'(x)$
\pagebreak

$\int xw(x)dx$
\pagebreak

$M\underline{x} = \underline{c}$
\pagebreak

$M$
\pagebreak

\[M = L \times U\]
\pagebreak

$L$
\pagebreak

$U$
\pagebreak

$M^{-1}A$
\pagebreak

$M^{-1}b$
\pagebreak

$3\times4$
\pagebreak

\[\begin{matrix}\text{Row major} & \text {Column major}\\ \begin{bmatrix}1&2&3\\4&5&6\\7&8&9\end{bmatrix} & \begin{bmatrix}1&4&7\\2&5&8\\3&6&9\end{bmatrix} \end{matrix}\]
\pagebreak

\[ AP = QR \]
\pagebreak

$P$
\pagebreak

$R$
\pagebreak

$i$
\pagebreak

$P(i)$
\pagebreak

$QR$
\pagebreak

$2\times 3$
\pagebreak

$\underline{x}$
\pagebreak

$\underline{x}'$
\pagebreak

\[\begin{aligned}\underline{x}' &= E\times\underline{x}\\ \begin{bmatrix}x'\\y'\end{bmatrix} &= \begin{pmatrix}r_{11} & r_{12} & t_1\\r_{21} & r_{22} & t_2\end{pmatrix}\begin{bmatrix}x\\y\\1\end{bmatrix}\end{aligned}\]
\pagebreak

$3\times$
\pagebreak

\[\begin{aligned}\underline{x}' &= E\times\underline{x}\\ \begin{bmatrix}x'\\y'\\z'\end{bmatrix} &= \begin{pmatrix}r_{11} & r_{12} & r_{13} & t_1\\r_{21} & r_{22} & r_{23} & t_2\\r_{31} & r_{32} & r_{33} & t_3\end{pmatrix}\begin{bmatrix}x\\y\\z\\1\end{bmatrix}\end{aligned}\]
\pagebreak

$ B $
\pagebreak

$ e^{\text{Adj}(v)} = Be^{v}B^{-1} $
\pagebreak

$\vec{w}$
\pagebreak

$ \theta = |\vec{w}|$
\pagebreak

$\frac{\sin \theta}{\theta}$
\pagebreak

$\frac{1 - \cos \theta}{\theta^2}$
\pagebreak

$ \sum_i w_iG_i$
\pagebreak

$3\times3$
\pagebreak

$ M $
\pagebreak

$Adj()$
\pagebreak

$ e^{\text{Adj}(v)} = Me^{v}M^{-1} $
\pagebreak

\[M = U \times D \times V^T\]
\pagebreak

$D$
\pagebreak

$V$
\pagebreak

\[M^{\dagger} = V \times D^{-1} \times U^T\]
\pagebreak

$D^{-1}$
\pagebreak

\[M = U \times \Lambda \times U^T\]
\pagebreak

$U^T = U^{-1}$
\pagebreak

$\Lambda$
\pagebreak

$Lambda^{-1}$
\pagebreak

$U^T$
\pagebreak

$\sigma^2 = \frac{1}{\text{val}}$
\pagebreak

$\sigma_i^2 = \frac{1}{\text{v}_i}$
\pagebreak

$m$
\pagebreak

$\frac{\partial\text{m}}{\partial\text{param}_i}$
\pagebreak

$\frac{\partial\text{m}_i}{\partial\text{param}_j}$
\pagebreak

$J^\dagger e$
\pagebreak

$J^{\mathsf T} e$
\pagebreak

$(J^{\mathsf T} J + P)^{-1}$
\pagebreak

\end{document}
